\let\negmedspace\undefined
\let\negthickspace\undefined
\documentclass[journal,12pt,twocolumn]{IEEEtran}
\usepackage{cite}
\usepackage{amsmath,amssymb,amsfonts,amsthm}
\usepackage{algorithmic}
\usepackage{graphicx}
\usepackage{textcomp}
\usepackage{xcolor}
\usepackage{txfonts}
\usepackage{listings}
\usepackage{enumitem}
\usepackage{mathtools}
\usepackage{gensymb}
\usepackage{comment}
\usepackage[breaklinks=true]{hyperref}
\usepackage{tkz-euclide} 
\usepackage{listings}
\usepackage{gvv}                                        
\def\inputGnumericTable{}                                 
\usepackage[latin1]{inputenc}                                
\usepackage{color}                                            
\usepackage{array}                                            
\usepackage{longtable}                                       
\usepackage{calc}                                             
\usepackage{multirow}                                         
\usepackage{hhline}                                           
\usepackage{ifthen}                                           
\usepackage{lscape}

\newtheorem{theorem}{Theorem}[section]
\newtheorem{problem}{Problem}
\newtheorem{proposition}{Proposition}[section]
\newtheorem{lemma}{Lemma}[section]
\newtheorem{corollary}[theorem]{Corollary}
\newtheorem{example}{Example}[section]
\newtheorem{definition}[problem]{Definition}
\newcommand{\BEQA}{\begin{eqnarray}}
\newcommand{\EEQA}{\end{eqnarray}}
\newcommand{\define}{\stackrel{\triangle}{=}}
\theoremstyle{remark}
\newtheorem{rem}{Remark}
\begin{document}
\bibliographystyle{IEEEtran}
\vspace{3cm}
\title{11.9.4.4}
\author{EE23BTECH11027 - K RAHUL$^{*}$% <-this % stops a space
}
\maketitle
\newpage
\bigskip
\renewcommand{\thefigure}{\theenumi}
\renewcommand{\thetable}{\theenumi}
%Derivation for the Z transform of a function $x(n) = \frac{1}{n+c}u(n)$, where $c \in \mathbb{R}$
\begin{align}\label{11027_eq1}
    x(n) &= \frac{1}{n+c} u(n),\text{where} \: c \in \mathbb{R}\\
    X(z) &= \sum_{n= -\infty}^{n= +\infty} x(n)z^{-n}\\
    &=\sum_{n = 0}^{n = +\infty} \frac{1}{n+c}z^{-n}\\
    &= z^c\sum_{n = 0}^{n = +\infty} \frac{1}{n+c}z^{-(n+c)}\\
    &= z^c(-log(1-Z^{-1}) - z^{-1}-\frac{z^{-2}}{2}-\frac{z^{-3}}{3} \ldots -\frac{z^{-(c-1)}}{c-1}))
\end{align}
\begin{align}\label{11027_eq2}
    d(n)&=\frac{1}{2\pi j} \oint _C z^{n+1}\ln{(1-z^{-1})}dz\\
    &=\frac{-1}{2\pi j} \oint _C z^{n+1}(z^{-1}+\frac{z^{-2}}{2} + \frac{z^{-3}}{3}+.. + \frac{z^{-(n+1)}}{n+1}+ \frac{z^{-(n+2}}{n+2}+.. dz\\
    &z=e^{jt}\\
    &=\frac{-1}{2\pi} \int_{0}^{2\pi} e^{(n+2)jt}(e^{-jt}+\frac{e^{-2jt}}{2} + \frac{e^{-3jt}}{3}+.. +\frac{z^{-(n+2}jt}{n+2}+.. dz\\
    &=\frac{-1}{n+2}
\end{align}

\begin{align}\label{11027_eq3}
    d(n)&= \frac{z^n}{1-z^{-1}}\\
    &= \lim_{x \to 1}z^{n+1} \text{(Residue Theorem)}\\
    &= 1
\end{align}
\end{document}
