\let\negmedspace\undefined
\let\negthickspace\undefined
\documentclass[journal,12pt,twocolumn]{IEEEtran}
\usepackage{cite}
\usepackage{amsmath,amssymb,amsfonts,amsthm}
\usepackage{algorithmic}
\usepackage{graphicx}
\usepackage{textcomp}
\usepackage{xcolor}
\usepackage{txfonts}
\usepackage{listings}
\usepackage{enumitem}
\usepackage{mathtools}
\usepackage{gensymb}
\usepackage{comment}
\usepackage[breaklinks=true]{hyperref}
\usepackage{tkz-euclide} 
\usepackage{listings}
\usepackage{gvv} 
\usepackage{verbatim}                                       
\def\inputGnumericTable{}                                 
\usepackage[latin1]{inputenc}                                
\usepackage{color}                                            
\usepackage{array}                                            
\usepackage{longtable}                                       
\usepackage{calc}                                             
\usepackage{multirow}                                         
\usepackage{hhline}                                           
\usepackage{ifthen}                                           
\usepackage{lscape}
\newtheorem{theorem}{Theorem}[section]
\newtheorem{problem}{Problem}
\newtheorem{proposition}{Proposition}[section]
\newtheorem{lemma}{Lemma}[section]
\newtheorem{corollary}[theorem]{Corollary}
\newtheorem{example}{Example}[section]
\newtheorem{definition}[problem]{Definition}
\newcommand{\BEQA}{\begin{eqnarray}}
\newcommand{\EEQA}{\end{eqnarray}}
\newcommand{\define}{\stackrel{\triangle}{=}}
\theoremstyle{remark}
\newtheorem{rem}{Remark}
\begin{document}
\bibliographystyle{IEEEtran}
\vspace{3cm}
\title{11.9.4.4}
\author{EE23BTECH11027 - K RAHUL$^{*}$% <-this % stops a space
}
\maketitle
\newpage
\bigskip
\renewcommand{\thefigure}{\theenumi}
\renewcommand{\thetable}{\theenumi}
\textbf{Derivations and results:} \\
\begin{table}[ht]
\input{tables/table_1.2}
\end{table}
\begin{align}
	%\label{Z_trans_pair}\\
	\delta\brak{n} &\system{Z} 1 \\
	\delta\brak{n+k} &\system{Z}z^{-k} ,\forall k\in \mathbb{R} \label{delta_func}
\end{align}
\begin{align}
        \log\brak{1-x} = -x - \frac{x^2}{2} - \frac{x^3}{3}-\frac{x^4}{4}- \ldots \label{log_expansion}
\end{align}
Let $x\brak{n}$ and $w\brak{n}$ be some expression as described in the table in discrete time domain, whose $Z$ transform, $X\brak{z}$ and $W\brak{z}$ respectively, shall be obtained for future reference.\\
\begin{align}
    \notag \text{For }  x\brak{n} = \frac{1}{n+c} &u\brak{n},\forall c \geq 2,c \in \mathbb{N}\\
    X\brak{z} &= \sum_{n= -\infty}^{n= +\infty} x\brak{n}z^{-n}\\
    &=\sum_{n = 0}^{n = +\infty} \frac{1}{n+c}z^{-n}\\
    &= z^c\sum_{n = 0}^{n = +\infty} \frac{1}{n+c}z^{-\brak{n+c}}
\end{align}
Using, \eqref{log_expansion}
\begin{align}
    X\brak{z}&= z^c \biggl(-\log\brak{1-z^{-1}}- z^{-1}\notag\\& -\frac{z^{-2}}{2}-\frac{z^{-3}}{3} - \ldots -\frac{z^{-(c-1)}}{c-1} \biggr)\ \forall c \geq 2, c \in \mathbb{N} \label{when_c_not_1}
\end{align} 

\begin{align}
	\notag \text{For } w\brak{n} = \frac{1}{n+1}&u\brak{n},\\
	W\brak{z} &=\sum_{n= -\infty}^{n= +\infty} w\brak{n}z^{-n}\\
	&= \sum_{n = 0}^{n = +\infty} \frac{1}{n+1}z^{-n}\\
	&= z\sum_{n = 0}^{n = +\infty} \frac{1}{n+1}z^{-\brak{n+1}} 
\end{align}
Using \eqref{log_expansion},
\begin{align}
	W\brak{z}&= -z\log\brak{1-z^{-1}} \label{when_c_equals_1}	
\end{align}
\\
Let $D\brak{z}$ be some expression as described in the table in $Z$ domain, whose inverse $Z$ transform, $d\brak{n}$ shall be obtained for future reference.\\

\begin{align}
	\notag \text{For } D\brak{z}&= z^{k}\log\brak{1-z^{-1}} \forall k \geq 1, k\in \mathbb{Z}\\
	D\brak{z}&= \brak{-z^{k-1} - \frac{1}{2}z^{k-2} - \frac{1}{3}z^{k-3} - \frac{1}{4}z^{k-4} - \ldots}
\end{align}
Using \eqref{delta_func},
\begin{align}
	d\brak{n} &= \biggl(-\delta\brak{n+k-1}  -\frac{1}{2}\delta\brak{n+k-2}  -\frac{1}{3}\delta\brak{n+k-3} \notag \\ &-\frac{1}{4}\delta\brak{n+k-4} - \ldots - \frac{1}{n+k}\delta\brak{0}-\ldots\biggr)\\
	&= \frac{-1}{n+k} u\brak{n} \label{11027_eq_log}
\end{align}
\\
\newpage
\textbf{Question:} \\
Find sum to n terms of the following series:\\
$\frac{1}{1 \times 2} + \frac{1}{2 \times 3} + \frac{1}{3 \times 4} + \ldots$
\bigskip \bigskip


\solution
\begin{table}[ht]
\input{tables/table_1.1}
\end{table}
\begin{align}
x\brak{n} &= \frac{1}{\brak{n+1}\brak{n+2}}u\brak{n}\\
& = \brak{\frac{1}{n+1} - \frac{1}{n+2}}u\brak{n}
\end{align}
Using \eqref{when_c_not_1} and \eqref{when_c_equals_1}, we get,
\begin{align}X\brak{z} &= -z log\brak{1-z^{-1}} + z^2 \log\brak{1-z^{-1}} + z\\
&= z\brak{z-1}\log\brak{1-z^{-1}} + z\\
    Y\brak{z} &= X\brak{z}U\brak{z}\\
     &=z^2\log\brak{1-z^{-1}} + \frac{z}{1-z^{-1}}
\end{align}
\begin{align}
	u\brak{n} &\system{Z} \frac{1}{1-z^{-1}} , \quad \abs{z} > 1\\
	u\brak{n+k} &\system{Z} \frac{z^k}{1-z^{-1}}, \forall k\in \mathbb{R}, \quad \abs{z} > 1 \label{Z_trans_pair}
\end{align}
Using \eqref{Z_trans_pair} and \eqref{11027_eq_log} ,
\begin{align}
    y\brak{n} &= u\brak{n+1} - \frac{1}{n+2}u\brak{n} , \; n \geq 0
\end{align}
Since $y(n)$ is only defined for $n \geq 0$, the above expression can be equivalently written as
\begin{align}
	y\brak{n} &= \brak{1-\frac{1}{n+2}} u\brak{n}
\end{align}
\newpage
\begin{figure}[h]
    %\caption{Stem Plot of $x\brak{n}$ v/s n}
    \includegraphics[width=0.3\textwidth]{figs/y(n)_vs_n.png}\label{fig:stem-plot}
    \caption{Stem Plot of $y\brak{n}$ v/s n}
\end{figure}
\end{document}


