\begin{table}[ht]
\input{tables/table_1.2}
\end{table}
\begin{align}
	u\brak{n} &\system{Z} \frac{1}{1-z^{-1}} , \quad \abs{z} > 1\\
	u\brak{n+k} &\system{Z} \frac{z^k}{1-z^{-1}}, \forall k\in \mathbb{R}, \quad \abs{z} > 1  \label{Z_trans_pair}\\
	\delta\brak{n} &\system{Z} 1 \\
	\delta\brak{n+k} &\system{Z}z^{-k} ,\forall k\in \mathbb{R} \label{11027_eq2}
\end{align}
\begin{align}
        \log\brak{1-x} = -x - \frac{x^2}{2} - \frac{x^3}{3}-\frac{x^4}{4}- \ldots \label{log_expansion}
\end{align}
Let $x\brak{n}$ and $w\brak{n}$ be some expression as described in the table in discrete time domain, whose $Z$ transform, $X\brak{z}$ and $W\brak{z}$ respectively, shall be obtained for future reference.\\
For  $x\brak{n} = \frac{1}{n+c} u\brak{n},\forall c \geq 2,c \in \mathbb{N}$
\begin{align}
    X\brak{z} &= \sum_{n= -\infty}^{n= +\infty} x\brak{n}z^{-n}\\
    &=\sum_{n = 0}^{n = +\infty} \frac{1}{n+c}z^{-n}\\
    &= z^c\sum_{n = 0}^{n = +\infty} \frac{1}{n+c}z^{-\brak{n+c}}
\end{align}
Using, \eqref{log_expansion}
\begin{align}
    X\brak{z}&= z^c \biggl(-\log\brak{1-z^{-1}}- z^{-1}\notag\\& -\frac{z^{-2}}{2}-\frac{z^{-3}}{3} - \ldots -\frac{z^{-(c-1)}}{c-1} \biggr)\ \forall c \geq 2, c \in \mathbb{N} \label{11027_eq1}
\end{align} 
For $w\brak{n} = \frac{1}{n+1}u\brak{n},$\\
\begin{align}
	W\brak{z} &=\sum_{n= -\infty}^{n= +\infty} w\brak{n}z^{-n}\\
	&= \sum_{n = 0}^{n = +\infty} \frac{1}{n+1}z^{-n}\\
	&= z\sum_{n = 0}^{n = +\infty} \frac{1}{n+1}z^{-\brak{n+1}} 
\end{align}
Using \eqref{log_expansion},
\begin{align}
	W\brak{z}&= -z\log\brak{1-z^{-1}} \label{When_c_equals_1}	
\end{align}
\\
Let $D\brak{z}$ be some expression as described in the table in $Z$ domain, whose inverse $Z$ transform, $d\brak{n}$ shall be obtained for future reference.\\
For $D\brak{z}= z^{k}\log\brak{1-z^{-1}} \forall k \geq 1, k\in \mathbb{Z}$
\begin{align}
	D\brak{z}&= \brak{-z^{k-1} - \frac{1}{2}z^{k-2} - \frac{1}{3}z^{k-3} - \frac{1}{4}z^{k-4} - \ldots}
\end{align}
Using \eqref{11027_eq2},
\begin{align}
	d\brak{n} &= \biggl(-\delta\brak{n+k-1}  -\frac{1}{2}\delta\brak{n+k-2}  -\frac{1}{3}\delta\brak{n+k-3} \notag \\ &-\frac{1}{4}\delta\brak{n+k-4} - \ldots - \frac{1}{n+k}\delta\brak{0}-\ldots\biggr)\\
	&= \frac{-1}{n+k} u\brak{n} \label{11027_eq_log}
\end{align}
