%Derivation for the Z transform of a function $x(n) = \frac{1}{n+c}u(n)$, where $c \in \mathbb{R}$
\begin{align}
        log\brak{1-x} = -x - \frac{x^2}{2} - \frac{x^3}{3}-\frac{x^4}{4}- \ldots \label{log_expansion}
\end{align}
Let $x\brak{n}$ be some expression in discrete time domain, whose $Z$ transform, $X(z)$ shall be obtained for future reference.\\
For  $x\brak{n} = \frac{1}{n+c} u\brak{n},\text{where} \: c \geq 2,\: c \in \mathbb{N}$\\
\begin{align}
    X\brak{z} &= \sum_{n= -\infty}^{n= +\infty} x\brak{n}z^{-n}\\
    &=\sum_{n = 0}^{n = +\infty} \frac{1}{n+c}z^{-n}\\
    &= z^c\sum_{n = 0}^{n = +\infty} \frac{1}{n+c}z^{-\brak{n+c}} \\
\end{align}
Using, \eqref{log_expansion}\\
\begin{align}
    X\brak{z}&= z^c \biggl(-log\brak{1-z^{-1}}- z^{-1}\notag\\& \;\;\;\;-\frac{z^{-2}}{2}-\frac{z^{-3}}{3} - \ldots -\frac{z^{-(c-1)}}{c-1} \biggr)\label{11027_eq1}
\end{align} 
For $x\brak{n} = \frac{1}{n+1}u\brak{n},$\\
\begin{align}
	X\brak{z} &=\sum_{n= -\infty}^{n= +\infty} x\brak{n}z^{-n}\\
	&= \sum_{n = 0}^{n = +\infty} \frac{1}{n+1}z^{-n}\\
	&= z\sum_{n = 0}^{n = +\infty} \frac{1}{n+1}z^{-\brak{n+1}} \\
\end{align}
Using \eqref{log_expansion},\\
\begin{align}
	X\brak{z}&= -zlog\brak{1-z^{-1}} \label{When_c_equals_1}	
\end{align}
\newpage

Let $D\brak{z}$ be some expression in $Z$ domain, whose inverse $Z$ transform, $d(n)$ shall be obtained for future reference.\\
For $D\brak{z}= z^{2}log\brak{1-z^{-1}}$
\begin{align}
    d\brak{n}&= \frac{1}{2\pi j} \oint _C z^{n+1}\log{\brak{1-z^{-1}}}dz\\
    &=\frac{-1}{2\pi j} \oint _C z^{n+1}\biggl(z^{-1}+\frac{z^{-2}}{2} + \frac{z^{-3}}{3}+\ldots \notag\\ \;\: &+ \frac{z^{-(n+1)}}{n+1} +  \frac{z^{-\brak{n+2}}}{n+2}+ \ldots \biggr) dz\\ 
\end{align}
Making the substitution $z=e^{jt} \implies dz = je^{jt}$
\begin{align}  
    d\brak{n}&=\frac{-1}{2\pi} \int_{0}^{2\pi} e^{\brak{n+2}jt}\biggl(e^{-jt}+\frac{e^{-2jt}}{2} \notag \\&+ \frac{e^{-3jt}}{3} +.. +\frac{z^{-\brak{n+2}}jt}{n+2}+..\biggr) dz\\
    &=\frac{-1}{n+2}\label{11027_eq2}
\end{align}
\\
\begin{align}
    \notag \text{For }D\brak{z}&= \frac{z^k}{1-z^{-1}},\text{where} \: k \in \mathbb{R}\\
    d\brak{n}&=\frac{1}{2\pi j} \oint _C \frac{z^{n+k-1}}{1-z^{-1}}dz
\end{align}
Using Residue Theorem,
\begin{align}
    d\brak{n}&= \lim_{z \to 1}\brak{\frac{z^{n+k-1}}{1-z^{-1}}}\brak{{1-z^{-1}}} \\
    &= 1\label{11027_eq3}
\end{align}

